DynamoDbEncryption/dafny/JsonEncryptor/Model/AwsCryptographyDbEncryptionSdkDynamoDbJsonTypes.dfy
@@ -2,360 +2,358 @@
 // SPDX-License-Identifier: Apache-2.0
 // Do not modify this file. This file is machine generated, and any changes to it will be overwritten.
 include "../../../../submodules/MaterialProviders/StandardLibrary/src/Index.dfy"
- include "../../StructuredEncryption/src/Index.dfy"
- include "../../../../submodules/MaterialProviders/AwsCryptographicMaterialProviders/dafny/AwsCryptographicMaterialProviders/src/Index.dfy"
- include "../../../../submodules/MaterialProviders/AwsCryptographyPrimitives/src/Index.dfy"
- module {:extern "software.amazon.cryptography.dbencryptionsdk.dynamodb.json.internaldafny.types" } AwsCryptographyDbEncryptionSdkDynamoDbJsonTypes
- {
- import opened Wrappers
- import opened StandardLibrary.UInt
- import opened UTF8
- import AwsCryptographyDbEncryptionSdkStructuredEncryptionTypes
- import AwsCryptographyMaterialProvidersTypes
- import AwsCryptographyPrimitivesTypes
- // Generic helpers for verification of mock/unit tests.
- datatype DafnyCallEvent<I, O> = DafnyCallEvent(input: I, output: O)
- 
- // Begin Generated Types
- 
- datatype Action =
- | crypto(crypto: AwsCryptographyDbEncryptionSdkStructuredEncryptionTypes.CryptoAction)
- | esdk(esdk: EsdkEncrypt)
- | dbesdk(dbesdk: DbesdkEncrypt)
- type AttributeActions = map<string, Action>
- type AttributeNameList = seq<string>
- datatype DbesdkEncrypt = | DbesdkEncrypt (
- nameonly keyring: Option<AwsCryptographyMaterialProvidersTypes.IKeyring> := Option.None ,
- nameonly cmm: Option<AwsCryptographyMaterialProvidersTypes.ICryptographicMaterialsManager> := Option.None ,
- nameonly algorithmSuiteId: Option<AwsCryptographyMaterialProvidersTypes.DBEAlgorithmSuiteId> := Option.None
- )
- datatype DecryptAs = | DecryptAs (
- nameonly encrypt: Option<string> := Option.None ,
- nameonly decrypt: Option<string> := Option.None
- )
- type DecryptAsList = seq<string>
- datatype DecryptObjectInput = | DecryptObjectInput (
- nameonly encryptedObject: Json
- )
- datatype DecryptObjectOutput = | DecryptObjectOutput (
- nameonly plaintextObject: Json ,
- nameonly parsedHeader: Option<ParsedHeader> := Option.None
- )
- datatype EncryptObjectInput = | EncryptObjectInput (
- nameonly plaintextObject: Json
- )
- datatype EncryptObjectOutput = | EncryptObjectOutput (
- nameonly encryptedObject: Json ,
- nameonly parsedHeader: Option<ParsedHeader> := Option.None
- )
- datatype EsdkEncrypt = | EsdkEncrypt (
- nameonly encryptionContext: Option<AwsCryptographyMaterialProvidersTypes.EncryptionContext> := Option.None ,
- nameonly materialsManager: Option<AwsCryptographyMaterialProvidersTypes.ICryptographicMaterialsManager> := Option.None ,
- nameonly keyring: Option<AwsCryptographyMaterialProvidersTypes.IKeyring> := Option.None ,
- nameonly algorithmSuiteId: Option<AwsCryptographyMaterialProvidersTypes.ESDKAlgorithmSuiteId> := Option.None ,
- nameonly frameLength: Option<FrameLength> := Option.None
- )
- type FrameLength = x: int64 | IsValid_FrameLength(x) witness *
- predicate method IsValid_FrameLength(x: int64) {
- ( 1 <= x <= 4294967296 )
-}
- datatype Json =
- | utf8(utf8: Utf8Bytes)
- | text(text: string)
- class IJsonEncryptorClientCallHistory {
- ghost constructor() {
- EncryptObject := [];
- DecryptObject := [];
-}
- ghost var EncryptObject: seq<DafnyCallEvent<EncryptObjectInput, Result<EncryptObjectOutput, Error>>>
- ghost var DecryptObject: seq<DafnyCallEvent<DecryptObjectInput, Result<DecryptObjectOutput, Error>>>
-}
- trait {:termination false} IJsonEncryptorClient
- {
- // Helper to define any additional modifies/reads clauses.
- // If your operations need to mutate state,
- // add it in your constructor function:
- // Modifies := {your, fields, here, History};
- // If you do not need to mutate anything:
-// Modifies := {History};
+include "../../StructuredEncryption/src/Index.dfy"
+include "../../../../submodules/MaterialProviders/AwsCryptographicMaterialProviders/dafny/AwsCryptographicMaterialProviders/src/Index.dfy"
+include "../../../../submodules/MaterialProviders/AwsCryptographyPrimitives/src/Index.dfy"
+module {:extern "software.amazon.cryptography.dbencryptionsdk.dynamodb.json.internaldafny.types" } AwsCryptographyDbEncryptionSdkDynamoDbJsonTypes
+{
+  import opened Wrappers
+  import opened StandardLibrary.UInt
+  import opened UTF8
+  import AwsCryptographyDbEncryptionSdkStructuredEncryptionTypes
+  import AwsCryptographyMaterialProvidersTypes
+  import AwsCryptographyPrimitivesTypes
+    // Generic helpers for verification of mock/unit tests.
+  datatype DafnyCallEvent<I, O> = DafnyCallEvent(input: I, output: O)
 
- ghost const Modifies: set<object>
- // For an unassigned field defined in a trait,
- // Dafny can only assign a value in the constructor.
- // This means that for Dafny to reason about this value,
- // it needs some way to know (an invariant),
- // about the state of the object.
- // This builds on the Valid/Repr paradigm
- // To make this kind requires safe to add
- // to methods called from unverified code,
- // the predicate MUST NOT take any arguments.
- // This means that the correctness of this requires
- // MUST only be evaluated by the class itself.
- // If you require any additional mutation,
- // then you MUST ensure everything you need in ValidState.
- // You MUST also ensure ValidState in your constructor.
- predicate ValidState()
- ensures ValidState() ==> History in Modifies
-  ghost const History: IJsonEncryptorClientCallHistory
- predicate EncryptObjectEnsuresPublicly(input: EncryptObjectInput , output: Result<EncryptObjectOutput, Error>)
- // The public method to be called by library consumers
- method EncryptObject ( input: EncryptObjectInput )
- returns (output: Result<EncryptObjectOutput, Error>)
- requires
- && ValidState()
- modifies Modifies - {History} ,
- History`EncryptObject
- // Dafny will skip type parameters when generating a default decreases clause.
- decreases Modifies - {History}
- ensures
- && ValidState()
- ensures EncryptObjectEnsuresPublicly(input, output)
- ensures History.EncryptObject == old(History.EncryptObject) + [DafnyCallEvent(input, output)]
- 
- predicate DecryptObjectEnsuresPublicly(input: DecryptObjectInput , output: Result<DecryptObjectOutput, Error>)
- // The public method to be called by library consumers
- method DecryptObject ( input: DecryptObjectInput )
- returns (output: Result<DecryptObjectOutput, Error>)
- requires
- && ValidState()
- modifies Modifies - {History} ,
- History`DecryptObject
- // Dafny will skip type parameters when generating a default decreases clause.
- decreases Modifies - {History}
- ensures
- && ValidState()
- ensures DecryptObjectEnsuresPublicly(input, output)
- ensures History.DecryptObject == old(History.DecryptObject) + [DafnyCallEvent(input, output)]
- 
-}
- datatype JsonEncryptorConfig = | JsonEncryptorConfig (
- nameonly logicalTableName: string ,
- nameonly attributeActionsOnEncrypt: AttributeActions ,
- nameonly allowedUnsignedAttributes: Option<AttributeNameList> := Option.None ,
- nameonly allowedUnsignedAttributePrefix: Option<string> := Option.None ,
- nameonly encrypt: DbesdkEncrypt ,
- nameonly decryptAs: Option<DecryptAsList> := Option.None
- )
- datatype ParsedHeader = | ParsedHeader (
- nameonly attributeActionsOnEncrypt: AttributeActions ,
- nameonly algorithmSuiteId: AwsCryptographyMaterialProvidersTypes.DBEAlgorithmSuiteId ,
- nameonly encryptedDataKeys: AwsCryptographyMaterialProvidersTypes.EncryptedDataKeyList ,
- nameonly storedEncryptionContext: AwsCryptographyMaterialProvidersTypes.EncryptionContext ,
- nameonly encryptionContext: AwsCryptographyMaterialProvidersTypes.EncryptionContext
- )
- type Utf8Bytes = ValidUTF8Bytes
- datatype Error =
- // Local Error structures are listed here
- | JsonEncryptorException (
- nameonly message: string
- )
- // Any dependent models are listed here
- | AwsCryptographyDbEncryptionSdkStructuredEncryption(AwsCryptographyDbEncryptionSdkStructuredEncryption: AwsCryptographyDbEncryptionSdkStructuredEncryptionTypes.Error)
- | AwsCryptographyMaterialProviders(AwsCryptographyMaterialProviders: AwsCryptographyMaterialProvidersTypes.Error)
- | AwsCryptographyPrimitives(AwsCryptographyPrimitives: AwsCryptographyPrimitivesTypes.Error)
- // The Collection error is used to collect several errors together
- // This is useful when composing OR logic.
- // Consider the following method:
- // 
- // method FN<I, O>(n:I)
- //   returns (res: Result<O, Types.Error>)
- //   ensures A(I).Success? ==> res.Success?
- //   ensures B(I).Success? ==> res.Success?
- //   ensures A(I).Failure? && B(I).Failure? ==> res.Failure?
- // 
- // If either A || B is successful then FN is successful.
- // And if A && B fail then FN will fail.
- // But what information should FN transmit back to the caller?
- // While it may be correct to hide these details from the caller,
- // this can not be the globally correct option.
- // Suppose that A and B can be blocked by different ACLs,
- // and that their representation of I is only eventually consistent.
- // How can the caller distinguish, at a minimum for logging,
- // the difference between the four failure modes?
- // || (!access(A(I)) && !access(B(I)))
- // || (!exit(A(I)) && !exit(B(I)))
- // || (!access(A(I)) && !exit(B(I)))
- // || (!exit(A(I)) && !access(B(I)))
- | CollectionOfErrors(list: seq<Error>, nameonly message: string)
- // The Opaque error, used for native, extern, wrapped or unknown errors
- | Opaque(obj: object)
- type OpaqueError = e: Error | e.Opaque? witness *
-}
- abstract module AbstractAwsCryptographyDbEncryptionSdkDynamoDbJsonService
- {
- import opened Wrappers
- import opened StandardLibrary.UInt
- import opened UTF8
- import opened Types = AwsCryptographyDbEncryptionSdkDynamoDbJsonTypes
- import Operations : AbstractAwsCryptographyDbEncryptionSdkDynamoDbJsonOperations
- function method DefaultJsonEncryptorConfig(): JsonEncryptorConfig
- method JsonEncryptor(config: JsonEncryptorConfig := DefaultJsonEncryptorConfig())
- returns (res: Result<IJsonEncryptorClient, Error>)
- requires config.encrypt.keyring.Some? ==>
- config.encrypt.keyring.value.ValidState()
- requires config.encrypt.cmm.Some? ==>
- config.encrypt.cmm.value.ValidState()
- requires var tmps0 := set t0 | t0 in config.attributeActionsOnEncrypt.Values;
- forall tmp0 :: tmp0 in tmps0 ==>
- tmp0.esdk? ==>
- tmp0.esdk.materialsManager.Some? ==>
- tmp0.esdk.materialsManager.value.ValidState()
- requires var tmps1 := set t1 | t1 in config.attributeActionsOnEncrypt.Values;
- forall tmp1 :: tmp1 in tmps1 ==>
- tmp1.esdk? ==>
- tmp1.esdk.keyring.Some? ==>
- tmp1.esdk.keyring.value.ValidState()
- modifies if config.encrypt.keyring.Some? then 
- config.encrypt.keyring.value.Modifies
- else {}
- modifies if config.encrypt.cmm.Some? then 
- config.encrypt.cmm.value.Modifies
- else {}
- modifies set tmps2 <- set t2 <- config.attributeActionsOnEncrypt.Values
-  | t2.esdk? && t2.esdk.materialsManager.Some? 
-  :: t2.esdk.materialsManager.value,
- obj <- tmps2.Modifies | obj in tmps2.Modifies :: obj
- modifies set tmps3 <- set t3 <- config.attributeActionsOnEncrypt.Values
-  | t3.esdk? 
-  && t3.esdk.keyring.Some? 
-  :: t3.esdk.keyring.value,
- obj <- tmps3.Modifies | obj in tmps3.Modifies :: obj
- ensures res.Success? ==> 
- && fresh(res.value)
- && fresh(res.value.Modifies
- - ( if config.encrypt.keyring.Some? then 
- config.encrypt.keyring.value.Modifies
- else {}
- ) - ( if config.encrypt.cmm.Some? then 
- config.encrypt.cmm.value.Modifies
- else {}
- ) - ( set tmps4 <- set t4 <- config.attributeActionsOnEncrypt.Values
-  | t4.esdk? 
-  && t4.esdk.materialsManager.Some? 
-  :: t4.esdk.materialsManager.value,
- obj <- tmps4.Modifies | obj in tmps4.Modifies :: obj
- ) - ( set tmps5 <- set t5 <- config.attributeActionsOnEncrypt.Values
-  | t5.esdk? 
-  && t5.esdk.keyring.Some? 
-  :: t5.esdk.keyring.value,
- obj <- tmps5.Modifies | obj in tmps5.Modifies :: obj
- ) )
- && fresh(res.value.History)
- && res.value.ValidState()
- ensures config.encrypt.keyring.Some? ==>
- config.encrypt.keyring.value.ValidState()
- ensures config.encrypt.cmm.Some? ==>
- config.encrypt.cmm.value.ValidState()
- ensures var tmps6 := set t6 | t6 in config.attributeActionsOnEncrypt.Values;
- forall tmp6 :: tmp6 in tmps6 ==>
- tmp6.esdk? ==>
- tmp6.esdk.materialsManager.Some? ==>
- tmp6.esdk.materialsManager.value.ValidState()
- ensures var tmps7 := set t7 | t7 in config.attributeActionsOnEncrypt.Values;
- forall tmp7 :: tmp7 in tmps7 ==>
- tmp7.esdk? ==>
- tmp7.esdk.keyring.Some? ==>
- tmp7.esdk.keyring.value.ValidState()
+  // Begin Generated Types
 
- // Helper function for the benefit of native code to create a Success(client) without referring to Dafny internals
- function method CreateSuccessOfClient(client: IJsonEncryptorClient): Result<IJsonEncryptorClient, Error> {
-   Success(client)
- } // Helper function for the benefit of native code to create a Failure(error) without referring to Dafny internals
- function method CreateFailureOfError(error: Error): Result<IJsonEncryptorClient, Error> {
-   Failure(error)
- }
- class JsonEncryptorClient extends IJsonEncryptorClient
- {
- constructor(config: Operations.InternalConfig)
- requires Operations.ValidInternalConfig?(config)
- ensures
- && ValidState()
- && fresh(History)
- && this.config == config
- const config: Operations.InternalConfig
- predicate ValidState()
- ensures ValidState() ==>
- && Operations.ValidInternalConfig?(config)
- && History !in Operations.ModifiesInternalConfig(config)
- && Modifies == Operations.ModifiesInternalConfig(config) + {History}
- predicate EncryptObjectEnsuresPublicly(input: EncryptObjectInput , output: Result<EncryptObjectOutput, Error>)
- {Operations.EncryptObjectEnsuresPublicly(input, output)}
- // The public method to be called by library consumers
- method EncryptObject ( input: EncryptObjectInput )
- returns (output: Result<EncryptObjectOutput, Error>)
- requires
- && ValidState()
- modifies Modifies - {History} ,
- History`EncryptObject
- // Dafny will skip type parameters when generating a default decreases clause.
- decreases Modifies - {History}
- ensures
- && ValidState()
- ensures EncryptObjectEnsuresPublicly(input, output)
- ensures History.EncryptObject == old(History.EncryptObject) + [DafnyCallEvent(input, output)]
- {
- output := Operations.EncryptObject(config, input);
- History.EncryptObject := History.EncryptObject + [DafnyCallEvent(input, output)];
+  datatype Action =
+    | crypto(crypto: AwsCryptographyDbEncryptionSdkStructuredEncryptionTypes.CryptoAction)
+    | esdk(esdk: EsdkEncrypt)
+    | dbesdk(dbesdk: JsonEncrypt)
+  type AttributeActions = map<string, Action>
+  type AttributeNameList = seq<string>
+  datatype DecryptObjectInput = | DecryptObjectInput (
+    nameonly encryptedObject: Json
+  )
+  datatype DecryptObjectOutput = | DecryptObjectOutput (
+    nameonly plaintextObject: Json ,
+    nameonly parsedHeader: Option<ParsedHeader> := Option.None
+  )
+  datatype EncryptObjectInput = | EncryptObjectInput (
+    nameonly plaintextObject: Json
+  )
+  datatype EncryptObjectOutput = | EncryptObjectOutput (
+    nameonly encryptedObject: Json ,
+    nameonly parsedHeader: Option<ParsedHeader> := Option.None
+  )
+  datatype EsdkEncrypt = | EsdkEncrypt (
+    nameonly encryptionContext: Option<AwsCryptographyMaterialProvidersTypes.EncryptionContext> := Option.None ,
+    nameonly materialsManager: Option<AwsCryptographyMaterialProvidersTypes.ICryptographicMaterialsManager> := Option.None ,
+    nameonly keyring: Option<AwsCryptographyMaterialProvidersTypes.IKeyring> := Option.None ,
+    nameonly algorithmSuiteId: Option<AwsCryptographyMaterialProvidersTypes.ESDKAlgorithmSuiteId> := Option.None ,
+    nameonly frameLength: Option<FrameLength> := Option.None
+  )
+  type FrameLength = x: int64 | IsValid_FrameLength(x) witness *
+  predicate method IsValid_FrameLength(x: int64) {
+    ( 1 <= x <= 4294967296 )
+  }
+  datatype Json =
+    | utf8(utf8: Utf8Bytes)
+    | text(text: string)
+  datatype JsonEncrypt = | JsonEncrypt (
+    nameonly keyring: Option<AwsCryptographyMaterialProvidersTypes.IKeyring> := Option.None ,
+    nameonly cmm: Option<AwsCryptographyMaterialProvidersTypes.ICryptographicMaterialsManager> := Option.None ,
+    nameonly algorithmSuiteId: Option<AwsCryptographyMaterialProvidersTypes.DBEAlgorithmSuiteId> := Option.None ,
+    nameonly signedValue: Option<SignedValues> := Option.None ,
+    nameonly encryptionContext: Option<AwsCryptographyMaterialProvidersTypes.EncryptionContext> := Option.None
+  )
+  class IJsonEncryptorClientCallHistory {
+    ghost constructor() {
+      EncryptObject := [];
+      DecryptObject := [];
+    }
+    ghost var EncryptObject: seq<DafnyCallEvent<EncryptObjectInput, Result<EncryptObjectOutput, Error>>>
+    ghost var DecryptObject: seq<DafnyCallEvent<DecryptObjectInput, Result<DecryptObjectOutput, Error>>>
+  }
+  trait {:termination false} IJsonEncryptorClient
+  {
+    // Helper to define any additional modifies/reads clauses.
+    // If your operations need to mutate state,
+    // add it in your constructor function:
+    // Modifies := {your, fields, here, History};
+    // If you do not need to mutate anything:
+    // Modifies := {History};
+
+    ghost const Modifies: set<object>
+    // For an unassigned field defined in a trait,
+    // Dafny can only assign a value in the constructor.
+    // This means that for Dafny to reason about this value,
+    // it needs some way to know (an invariant),
+    // about the state of the object.
+    // This builds on the Valid/Repr paradigm
+    // To make this kind requires safe to add
+    // to methods called from unverified code,
+    // the predicate MUST NOT take any arguments.
+    // This means that the correctness of this requires
+    // MUST only be evaluated by the class itself.
+    // If you require any additional mutation,
+    // then you MUST ensure everything you need in ValidState.
+    // You MUST also ensure ValidState in your constructor.
+    predicate ValidState()
+      ensures ValidState() ==> History in Modifies
+    ghost const History: IJsonEncryptorClientCallHistory
+    predicate EncryptObjectEnsuresPublicly(input: EncryptObjectInput , output: Result<EncryptObjectOutput, Error>)
+    // The public method to be called by library consumers
+    method EncryptObject ( input: EncryptObjectInput )
+      returns (output: Result<EncryptObjectOutput, Error>)
+      requires
+        && ValidState()
+      modifies Modifies - {History} ,
+               History`EncryptObject
+      // Dafny will skip type parameters when generating a default decreases clause.
+      decreases Modifies - {History}
+      ensures
+        && ValidState()
+      ensures EncryptObjectEnsuresPublicly(input, output)
+      ensures History.EncryptObject == old(History.EncryptObject) + [DafnyCallEvent(input, output)]
+
+    predicate DecryptObjectEnsuresPublicly(input: DecryptObjectInput , output: Result<DecryptObjectOutput, Error>)
+    // The public method to be called by library consumers
+    method DecryptObject ( input: DecryptObjectInput )
+      returns (output: Result<DecryptObjectOutput, Error>)
+      requires
+        && ValidState()
+      modifies Modifies - {History} ,
+               History`DecryptObject
+      // Dafny will skip type parameters when generating a default decreases clause.
+      decreases Modifies - {History}
+      ensures
+        && ValidState()
+      ensures DecryptObjectEnsuresPublicly(input, output)
+      ensures History.DecryptObject == old(History.DecryptObject) + [DafnyCallEvent(input, output)]
+
+  }
+  datatype JsonEncryptorConfig = | JsonEncryptorConfig (
+    nameonly domain: string ,
+    nameonly attributeActionsOnEncrypt: AttributeActions ,
+    nameonly allowedUnsignedAttributes: Option<AttributeNameList> := Option.None ,
+    nameonly allowedUnsignedAttributePrefix: Option<string> := Option.None ,
+    nameonly encrypt: JsonEncrypt
+  )
+  datatype ParsedHeader = | ParsedHeader (
+    nameonly attributeActionsOnEncrypt: AttributeActions ,
+    nameonly algorithmSuiteId: AwsCryptographyMaterialProvidersTypes.DBEAlgorithmSuiteId ,
+    nameonly encryptedDataKeys: AwsCryptographyMaterialProvidersTypes.EncryptedDataKeyList ,
+    nameonly storedEncryptionContext: AwsCryptographyMaterialProvidersTypes.EncryptionContext ,
+    nameonly encryptionContext: AwsCryptographyMaterialProvidersTypes.EncryptionContext
+  )
+  type SignedValues = map<string, string>
+  type Utf8Bytes = ValidUTF8Bytes
+  datatype Error =
+      // Local Error structures are listed here
+    | JsonEncryptorException (
+        nameonly message: string
+      )
+      // Any dependent models are listed here
+    | AwsCryptographyDbEncryptionSdkStructuredEncryption(AwsCryptographyDbEncryptionSdkStructuredEncryption: AwsCryptographyDbEncryptionSdkStructuredEncryptionTypes.Error)
+    | AwsCryptographyMaterialProviders(AwsCryptographyMaterialProviders: AwsCryptographyMaterialProvidersTypes.Error)
+    | AwsCryptographyPrimitives(AwsCryptographyPrimitives: AwsCryptographyPrimitivesTypes.Error)
+      // The Collection error is used to collect several errors together
+      // This is useful when composing OR logic.
+      // Consider the following method:
+      // 
+      // method FN<I, O>(n:I)
+      //   returns (res: Result<O, Types.Error>)
+      //   ensures A(I).Success? ==> res.Success?
+      //   ensures B(I).Success? ==> res.Success?
+      //   ensures A(I).Failure? && B(I).Failure? ==> res.Failure?
+      // 
+      // If either A || B is successful then FN is successful.
+      // And if A && B fail then FN will fail.
+      // But what information should FN transmit back to the caller?
+      // While it may be correct to hide these details from the caller,
+      // this can not be the globally correct option.
+      // Suppose that A and B can be blocked by different ACLs,
+      // and that their representation of I is only eventually consistent.
+      // How can the caller distinguish, at a minimum for logging,
+      // the difference between the four failure modes?
+    // || (!access(A(I)) && !access(B(I)))
+    // || (!exit(A(I)) && !exit(B(I)))
+    // || (!access(A(I)) && !exit(B(I)))
+    // || (!exit(A(I)) && !access(B(I)))
+    | CollectionOfErrors(list: seq<Error>, nameonly message: string)
+      // The Opaque error, used for native, extern, wrapped or unknown errors
+    | Opaque(obj: object)
+  type OpaqueError = e: Error | e.Opaque? witness *
 }
- 
- predicate DecryptObjectEnsuresPublicly(input: DecryptObjectInput , output: Result<DecryptObjectOutput, Error>)
- {Operations.DecryptObjectEnsuresPublicly(input, output)}
- // The public method to be called by library consumers
- method DecryptObject ( input: DecryptObjectInput )
- returns (output: Result<DecryptObjectOutput, Error>)
- requires
- && ValidState()
- modifies Modifies - {History} ,
- History`DecryptObject
- // Dafny will skip type parameters when generating a default decreases clause.
- decreases Modifies - {History}
- ensures
- && ValidState()
- ensures DecryptObjectEnsuresPublicly(input, output)
- ensures History.DecryptObject == old(History.DecryptObject) + [DafnyCallEvent(input, output)]
- {
- output := Operations.DecryptObject(config, input);
- History.DecryptObject := History.DecryptObject + [DafnyCallEvent(input, output)];
+abstract module AbstractAwsCryptographyDbEncryptionSdkDynamoDbJsonService
+{
+  import opened Wrappers
+  import opened StandardLibrary.UInt
+  import opened UTF8
+  import opened Types = AwsCryptographyDbEncryptionSdkDynamoDbJsonTypes
+  import Operations : AbstractAwsCryptographyDbEncryptionSdkDynamoDbJsonOperations
+  function method DefaultJsonEncryptorConfig(): JsonEncryptorConfig
+  method JsonEncryptor(config: JsonEncryptorConfig := DefaultJsonEncryptorConfig())
+    returns (res: Result<IJsonEncryptorClient, Error>)
+    requires config.encrypt.keyring.Some? ==>
+               config.encrypt.keyring.value.ValidState()
+    requires config.encrypt.cmm.Some? ==>
+               config.encrypt.cmm.value.ValidState()
+    requires var tmps0 := set t0 | t0 in config.attributeActionsOnEncrypt.Values;
+             forall tmp0 :: tmp0 in tmps0 ==>
+                              tmp0.esdk? ==>
+                                tmp0.esdk.materialsManager.Some? ==>
+                                  tmp0.esdk.materialsManager.value.ValidState()
+    requires var tmps1 := set t1 | t1 in config.attributeActionsOnEncrypt.Values;
+             forall tmp1 :: tmp1 in tmps1 ==>
+                              tmp1.esdk? ==>
+                                tmp1.esdk.keyring.Some? ==>
+                                  tmp1.esdk.keyring.value.ValidState()
+    modifies if config.encrypt.keyring.Some? then
+               config.encrypt.keyring.value.Modifies
+             else {}
+    modifies if config.encrypt.cmm.Some? then
+               config.encrypt.cmm.value.Modifies
+             else {}
+    modifies set tmps2 <- set t2 <- config.attributeActionsOnEncrypt.Values
+                                    | t2.esdk?
+                              && t2.esdk.materialsManager.Some?
+                            :: t2.esdk.materialsManager.value,
+               obj <- tmps2.Modifies | obj in tmps2.Modifies :: obj
+    modifies set tmps3 <- set t3 <- config.attributeActionsOnEncrypt.Values
+                                    | t3.esdk?
+                              && t3.esdk.keyring.Some?
+                            :: t3.esdk.keyring.value,
+               obj <- tmps3.Modifies | obj in tmps3.Modifies :: obj
+    ensures res.Success? ==>
+              && fresh(res.value)
+              && fresh(res.value.Modifies
+                       - ( if config.encrypt.keyring.Some? then
+                             config.encrypt.keyring.value.Modifies
+                           else {}
+                       ) - ( if config.encrypt.cmm.Some? then
+                               config.encrypt.cmm.value.Modifies
+                             else {}
+                       ) - ( set tmps4 <- set t4 <- config.attributeActionsOnEncrypt.Values
+                                                    | t4.esdk?
+                                              && t4.esdk.materialsManager.Some?
+                                            :: t4.esdk.materialsManager.value,
+                               obj <- tmps4.Modifies | obj in tmps4.Modifies :: obj
+                       ) - ( set tmps5 <- set t5 <- config.attributeActionsOnEncrypt.Values
+                                                    | t5.esdk?
+                                              && t5.esdk.keyring.Some?
+                                            :: t5.esdk.keyring.value,
+                               obj <- tmps5.Modifies | obj in tmps5.Modifies :: obj
+                       ) )
+              && fresh(res.value.History)
+              && res.value.ValidState()
+    ensures config.encrypt.keyring.Some? ==>
+              config.encrypt.keyring.value.ValidState()
+    ensures config.encrypt.cmm.Some? ==>
+              config.encrypt.cmm.value.ValidState()
+    ensures var tmps6 := set t6 | t6 in config.attributeActionsOnEncrypt.Values;
+            forall tmp6 :: tmp6 in tmps6 ==>
+                             tmp6.esdk? ==>
+                               tmp6.esdk.materialsManager.Some? ==>
+                                 tmp6.esdk.materialsManager.value.ValidState()
+    ensures var tmps7 := set t7 | t7 in config.attributeActionsOnEncrypt.Values;
+            forall tmp7 :: tmp7 in tmps7 ==>
+                             tmp7.esdk? ==>
+                               tmp7.esdk.keyring.Some? ==>
+                                 tmp7.esdk.keyring.value.ValidState()
+
+  // Helper function for the benefit of native code to create a Success(client) without referring to Dafny internals
+  function method CreateSuccessOfClient(client: IJsonEncryptorClient): Result<IJsonEncryptorClient, Error> {
+    Success(client)
+  } // Helper function for the benefit of native code to create a Failure(error) without referring to Dafny internals
+  function method CreateFailureOfError(error: Error): Result<IJsonEncryptorClient, Error> {
+    Failure(error)
+  }
+  class JsonEncryptorClient extends IJsonEncryptorClient
+  {
+    constructor(config: Operations.InternalConfig)
+      requires Operations.ValidInternalConfig?(config)
+      ensures
+        && ValidState()
+        && fresh(History)
+        && this.config == config
+    const config: Operations.InternalConfig
+    predicate ValidState()
+      ensures ValidState() ==>
+                && Operations.ValidInternalConfig?(config)
+                && History !in Operations.ModifiesInternalConfig(config)
+                && Modifies == Operations.ModifiesInternalConfig(config) + {History}
+    predicate EncryptObjectEnsuresPublicly(input: EncryptObjectInput , output: Result<EncryptObjectOutput, Error>)
+    {Operations.EncryptObjectEnsuresPublicly(input, output)}
+    // The public method to be called by library consumers
+    method EncryptObject ( input: EncryptObjectInput )
+      returns (output: Result<EncryptObjectOutput, Error>)
+      requires
+        && ValidState()
+      modifies Modifies - {History} ,
+               History`EncryptObject
+      // Dafny will skip type parameters when generating a default decreases clause.
+      decreases Modifies - {History}
+      ensures
+        && ValidState()
+      ensures EncryptObjectEnsuresPublicly(input, output)
+      ensures History.EncryptObject == old(History.EncryptObject) + [DafnyCallEvent(input, output)]
+    {
+      output := Operations.EncryptObject(config, input);
+      History.EncryptObject := History.EncryptObject + [DafnyCallEvent(input, output)];
+    }
+
+    predicate DecryptObjectEnsuresPublicly(input: DecryptObjectInput , output: Result<DecryptObjectOutput, Error>)
+    {Operations.DecryptObjectEnsuresPublicly(input, output)}
+    // The public method to be called by library consumers
+    method DecryptObject ( input: DecryptObjectInput )
+      returns (output: Result<DecryptObjectOutput, Error>)
+      requires
+        && ValidState()
+      modifies Modifies - {History} ,
+               History`DecryptObject
+      // Dafny will skip type parameters when generating a default decreases clause.
+      decreases Modifies - {History}
+      ensures
+        && ValidState()
+      ensures DecryptObjectEnsuresPublicly(input, output)
+      ensures History.DecryptObject == old(History.DecryptObject) + [DafnyCallEvent(input, output)]
+    {
+      output := Operations.DecryptObject(config, input);
+      History.DecryptObject := History.DecryptObject + [DafnyCallEvent(input, output)];
+    }
+
+  }
 }
- 
-}
-}
- abstract module AbstractAwsCryptographyDbEncryptionSdkDynamoDbJsonOperations {
- import opened Wrappers
- import opened StandardLibrary.UInt
- import opened UTF8
- import opened Types = AwsCryptographyDbEncryptionSdkDynamoDbJsonTypes
- type InternalConfig
- predicate ValidInternalConfig?(config: InternalConfig)
- function ModifiesInternalConfig(config: InternalConfig): set<object>
- predicate EncryptObjectEnsuresPublicly(input: EncryptObjectInput , output: Result<EncryptObjectOutput, Error>)
- // The private method to be refined by the library developer
+abstract module AbstractAwsCryptographyDbEncryptionSdkDynamoDbJsonOperations {
+  import opened Wrappers
+  import opened StandardLibrary.UInt
+  import opened UTF8
+  import opened Types = AwsCryptographyDbEncryptionSdkDynamoDbJsonTypes
+  type InternalConfig
+  predicate ValidInternalConfig?(config: InternalConfig)
+  function ModifiesInternalConfig(config: InternalConfig): set<object>
+  predicate EncryptObjectEnsuresPublicly(input: EncryptObjectInput , output: Result<EncryptObjectOutput, Error>)
+  // The private method to be refined by the library developer
 
 
- method EncryptObject ( config: InternalConfig , input: EncryptObjectInput )
- returns (output: Result<EncryptObjectOutput, Error>)
- requires
- && ValidInternalConfig?(config)
- modifies ModifiesInternalConfig(config)
- // Dafny will skip type parameters when generating a default decreases clause.
- decreases ModifiesInternalConfig(config)
- ensures
- && ValidInternalConfig?(config)
- ensures EncryptObjectEnsuresPublicly(input, output)
+  method EncryptObject ( config: InternalConfig , input: EncryptObjectInput )
+    returns (output: Result<EncryptObjectOutput, Error>)
+    requires
+      && ValidInternalConfig?(config)
+    modifies ModifiesInternalConfig(config)
+    // Dafny will skip type parameters when generating a default decreases clause.
+    decreases ModifiesInternalConfig(config)
+    ensures
+      && ValidInternalConfig?(config)
+    ensures EncryptObjectEnsuresPublicly(input, output)
 
 
- predicate DecryptObjectEnsuresPublicly(input: DecryptObjectInput , output: Result<DecryptObjectOutput, Error>)
- // The private method to be refined by the library developer
+  predicate DecryptObjectEnsuresPublicly(input: DecryptObjectInput , output: Result<DecryptObjectOutput, Error>)
+  // The private method to be refined by the library developer
 
 
- method DecryptObject ( config: InternalConfig , input: DecryptObjectInput )
- returns (output: Result<DecryptObjectOutput, Error>)
- requires
- && ValidInternalConfig?(config)
- modifies ModifiesInternalConfig(config)
- // Dafny will skip type parameters when generating a default decreases clause.
- decreases ModifiesInternalConfig(config)
- ensures
- && ValidInternalConfig?(config)
- ensures DecryptObjectEnsuresPublicly(input, output)
+  method DecryptObject ( config: InternalConfig , input: DecryptObjectInput )
+    returns (output: Result<DecryptObjectOutput, Error>)
+    requires
+      && ValidInternalConfig?(config)
+    modifies ModifiesInternalConfig(config)
+    // Dafny will skip type parameters when generating a default decreases clause.
+    decreases ModifiesInternalConfig(config)
+    ensures
+      && ValidInternalConfig?(config)
+    ensures DecryptObjectEnsuresPublicly(input, output)
 }
