DynamoDbEncryption/dafny/JsonEncryptor/src/JsonToStruct.dfy
@@ -5,6 +5,35 @@ include "../Model/AwsCryptographyDbEncryptionSdkDynamoDbJsonTypes.dfy"
 include "Util.dfy"
 
 module JsonToStruct {
+  export Fun
+  provides
+    ObjectToStructured,
+    StructuredToObject,
+    SmithyJsonToObject,
+    JsonToSmithyJson,
+    Wrappers,
+    Values,
+    SE,
+    AwsCryptographyDbEncryptionSdkDynamoDbJsonTypes,
+    MapKeysMatchItems,
+    SimplifyMapValueSuccess,
+    FindItem,
+    StandardLibrary,
+    OneBadResult,
+    JsonEncryptorUtil,
+    AttrToStructured,
+    StructuredToAttr,
+    JsonEqual
+  reveals
+    FlattenValueMap,
+    FlattenErrors,
+    SimplifyMapValue,
+    MapError,
+    MakeError,
+    StructuredDataTerminalType,
+    TerminalDataMap
+
+
   import opened Wrappers
   import opened StandardLibrary
   import opened StandardLibrary.UInt
@@ -20,8 +49,8 @@ module JsonToStruct {
 
   import JSON.Spec
   import JSON.API
-  import opened JSON.Values
   import JSON.Errors
+  import opened JSON.Values
 
   type StructuredDataTerminalType = x : SE.StructuredData | x.content.Terminal? witness *
   type TerminalDataMap = map<string, StructuredDataTerminalType>
@@ -95,26 +124,7 @@ module JsonToStruct {
   const MAP        : SE.TerminalTypeId := [MAP_T,  NULL_T]
   const LIST       : SE.TerminalTypeId := [LIST_T, NULL_T]
 
-
-  method SmithyJsonToObject(item : Json) returns (res :Result<JSON, string>)
-    ensures res.Success? ==> res.value.Object?
-  {
-    var json :- if item.text? then
-      StringToJson(item.text)
-    else
-      Utf8ToJson(item.utf8);
-
-    :- Need(json.Object?, "JSON to encrypt/decrypt must be an Object : " + SmithyJsonToString(item));
-    return Success(json);
-  }
-
-  function method {:opaque} SmithyJsonToObjectYYY(item : Json) : (res :Result<JSON, string>)
-    ensures res.Success? ==> res.value.Object?
-  {
-    SmithyJsonToObjectXXX(item)
-  }
-
-  function method {:opaque} SmithyJsonToObjectXXX(item : Json) : (res :Result<JSON, string>)
+  function method {:opaque} SmithyJsonToObject(item : Json) : (res :Result<JSON, string>)
     ensures res.Success? ==> res.value.Object?
   {
     var json :- if item.text? then
@@ -126,18 +136,7 @@ module JsonToStruct {
     Success(json)
   }
 
-  method JsonToSmithyJson(item : JSON, example : Json) returns (res : Result<Json, string>)
-  {
-    var jsonBytes :- API.Serialize(item).MapFailure((e : Errors.SerializationError) => e.ToString());
-    if example.utf8? {
-      return Success(utf8(example.utf8));
-    } else {
-      var textStr :- UTF8.Decode(jsonBytes);
-      return Success(text(textStr));
-    }
-  }
-
-  function method {:opaque} JsonToSmithyJsonXXX(item : JSON, example : Json) : Result<Json, string>
+  function method {:opaque} JsonToSmithyJson(item : JSON, example : Json) : Result<Json, string>
   {
     var jsonBytes :- API.Serialize(item).MapFailure((e : Errors.SerializationError) => e.ToString());
     if example.utf8? then
